check_fo with mut_excl TODO: all_but_last for cut

theories/check_fo.v
@@ -2,7 +2,14 @@ From det Require Import prelude.
 From mathcomp Require Import all_ssreflect.
 From det Require Import tree tree_prop ctx.
 
+Definition has_cut_seq:= (has (fun x => cut == x)).
+
 Section checker.
+  Fixpoint all_but_last {T : Type} P (l : seq T) :=
+    match l with 
+    | [::] | (_ :: [::]) => true
+    | x :: xs => P x && all_but_last P xs
+    end.
 
   Fixpoint is_det_sig (sig:S) : bool :=
     match sig with
@@ -18,16 +25,9 @@ Section checker.
     | Callable_App hd _ => getS_Callable sP hd
     end.
 
-  Fixpoint callable_is_det (sP: sigT) (t:Callable) : bool :=
-    match t with
-    | Callable_App h _ => callable_is_det sP h
-    | Callable_P k => 
-      if sP.[?k] is Some s then is_det_sig s
-      else false
-    end.
-
   Definition tm_is_det (sP: sigT) (t : Callable) :=
-    odflt false (omap is_det_sig (getS_Callable sP t)).
+    if getS_Callable sP t is Some s then is_det_sig s
+    else false.
 
   Definition check_atom sP (a: A) :=
     match a with
@@ -35,42 +35,205 @@ Section checker.
     | call t => tm_is_det sP t
     end. 
 
-  (* Definition not_same_head u p r1 r2 :=
-      exists i, input_pos i r1 = i1 -> input_pos i r2 = i2 ->
-         u.unif empty i1 i2 = None.
-
-          Axiom:
-  unif empty a b = None ->
-    forall s, match s a t = Some -> match s b t = None.
-
-  Lemma not_same_head_backchain :
-    not_same_head u p r1 r2 ->
-    let rl := (bc u p fv c s).2 in
-    r1 \in rl -> r2 \notin rl.
- *)
-
   (* There is cut and after the cut there are only call to Det preds *)
   Fixpoint check_atoms (sP :sigT) (s: seq A) :=
     match s with
-    | [::] => false
+    | [::] => true
     | cut :: xs => all (check_atom sP) xs || check_atoms sP xs
-    | call _ :: xs => check_atoms sP xs
+    | call c :: xs => (tm_is_det sP c || has_cut_seq xs) && check_atoms sP xs
     end.
 
   Definition check_rule sP head prems :=
-    (callable_is_det sP head == false) || 
+    (tm_is_det sP head == false) || 
       check_atoms sP prems.
 
   Definition check_rules sP rules :=
     all (fun x => check_rule sP x.(head) x.(premises)) rules.
-
-  Definition check_program sP pr := 
-    check_rules sP (rules pr).
 End checker.
 
-Definition has_cut_seq:= (has (fun x => cut == x)).
+Lemma tiki_taka sP s s3 modes t q pn hd1 u:
+  let t' := tm2RC (deref s (Callable2Tm t)) in
+  t' = Some (q, pn) ->
+  tm_is_det sP t ->
+    H u modes q hd1 s = Some s3 ->
+      tm_is_det sP hd1.
+Proof.
+  move=>/=.
+  elim: modes q pn hd1 t s s3 => //=.
+    move=> []//=k kp hd1 t s1 s2.
+    case: hd1 => //={}k0.
+    case: eqP => //=?; subst k0.
+    move=> ++ [?]; subst.
+    destruct t => //=; last by case: tm2RC => //=[[]].
+    by move=> [->->]/=; rewrite/tm_is_det/=; case: fndP.
+  move=> m //ml IH q pn hd t s1 s2 H1 H2 H3.
+  have {H3}: exists f1 a1 f2 a2,
+    q = Callable_App f1 a1 /\
+    hd = Callable_App f2 a2 /\
+    (obind (matching u a1 a2) (H u ml f1 f2 s1) = Some s2 \/
+    obind (unify u a1 a2) (H u ml f1 f2 s1) = Some s2).
+  by move: H3; destruct m, q, hd => //; repeat eexists; auto.
+  move=> [f1 [a1 [f2 [a2 [?[?]]]]]]; subst.
+  case e: H => //=[s3|]; last by case.
+  move: H2; rewrite/tm_is_det/=.
+  case: t H1 => //= c t.
+  case H : tm2RC => //=[[h1' hp]] [??]?; subst => /=.
+  case X: getS_Callable => //[S] H1/= H2.
+  by apply: IH H _ e; rewrite/tm_is_det X//.
+Qed.
+
+Section mut_excl.
+  Variable u : Unif.
+  (* Variable p : program. *)
+
+  Fixpoint H_head s (ml : list mode) (q : Callable) (h: Callable) : option Sigma :=
+    match ml,q,h with
+    | [::], Callable_P c, Callable_P c1 => if c == c1 then Some s else None
+    | [:: i & ml], (Callable_App q a1), (Callable_App h a2) => obind (u.(unify) a1 a2) (H_head s ml q h)
+    | [:: o & ml], (Callable_App q a1), (Callable_App h a2) => (H_head s ml q h)
+    | _, _, _ => None
+    end.
+  
+  Definition unif_head := H_head empty.
+
+  Fixpoint select_head (query : Callable) (modes:list mode) (rules: list R) : (seq R) :=
+    match rules with
+    | [::] => [::]
+    | rule :: rules =>
+      let tl := select_head query modes rules in
+      if H_head empty modes query rule.(head) then rule :: tl else tl
+    end.
+  
+  Definition mut_excl_head (sig:sigT) (query:Callable) rules :=
+    match tm2RC (Callable2Tm query) with
+      | None => true (*a callable against a non rigid term is OK: failure at runtime*)
+      | Some (query, kp) =>
+        match sig.[? kp] with 
+          | Some sig => 
+            if is_det_sig sig then 
+              let r := select_head query (get_modes_rev query sig) rules in
+              all (fun x => has_cut_seq x.(premises)) r
+            (* ignoring checking for vars *)
+            else true
+          (*a callable against a rigid term non in sig OK: failure at runtime*)
+          | None => true
+          end
+      end.
+
+  Lemma head_fresh_rule fv r:
+    head (fresh_rule fv r).2 = (fresh_callable fv r.(head)).2.
+  Proof.
+    destruct r; rewrite/fresh_rule/= 1!push.
+    case bc: fresh_atoms => [fv' A']//=.
+  Qed.
+
+  Lemma head_fresh_premises fv r:
+    premises (fresh_rule fv r).2 = (fresh_atoms (fresh_callable fv r.(head)).1 r.(premises)).2.
+  Proof.
+    destruct r; rewrite/fresh_rule/= 1!push.
+    generalize (fresh_callable fv head) => -[{}fv/=b].
+    case FA: fresh_atoms => [b1 a']//=.
+  Qed.
+
+  Lemma callable_is_det_fresh sP fv hd:
+    tm_is_det sP (fresh_callable fv hd).2 =
+      tm_is_det sP hd.
+  Proof.
+    rewrite/tm_is_det.
+    elim: hd fv => //= a Ha t fv.
+    by rewrite !push/= -(Ha fv).
+  Qed.
+
+  Lemma tm_is_det_comb sP f a:
+    tm_is_det sP (Callable_App f a) = tm_is_det sP f.
+  Proof. by rewrite/tm_is_det/=. Qed.
+  
+  Lemma tm_is_det_fresh sP c c' sv sv':
+    tm_is_det sP c ->
+    fresh_callable sv c = (sv', c') ->
+    tm_is_det sP c'.
+  Proof.
+    elim: c c' sv sv' => //=.
+      by move=> k c' sv sv' + [_ <-]//.
+    move=> f Hf a c' sv sv'.
+    case X: fresh_callable => [sv2 f'].
+    case Y: rename => [sv3 a'] + [_ <-].
+    rewrite !tm_is_det_comb => H.
+    by apply/Hf/X.
+  Qed.
+
+  Lemma fresh_has_cut sv xs sv' xs':
+    has_cut_seq xs -> fresh_atoms sv xs = (sv', xs') -> has_cut_seq xs'.
+  Proof.
+    elim: xs sv xs' sv' => //= x xs IH sv xs' sv'.
+    case Fs: fresh_atoms => [b' a'].
+    case Fa: fresh_atom => [b2 a2]/=+[_<-]/=.
+    move=> /orP [/eqP?|]; subst; first by move: Fa => /=[_<-].
+    by move=> H; rewrite (IH _ _ _ H Fs) orbT.
+  Qed.
+
+  Lemma check_atom_fresh sP x x' sv sv':
+    check_atom sP x ->
+    fresh_atom sv x = (sv', x') ->
+    check_atom sP x'.
+  Proof.
+    destruct x => //=; first by move=> _ [_ <-].
+    case X: fresh_callable => [svE c'] H [_ <-]/=.
+    by apply/tm_is_det_fresh/X.
+  Qed.
+
+  Lemma all_check_atom_fresh sP xs xs' sv sv':
+    all (check_atom sP) xs ->
+    fresh_atoms sv xs = (sv', xs') ->
+    all (check_atom sP) xs'.
+  Proof.
+    elim: xs xs' sv sv' => //=; first by move=> > _ [_ <-].
+    move=> x xs IH xsE sv svE /andP[H1 H2].
+    case Fs: fresh_atoms => [sv' xs'].
+    case Fa: fresh_atom => [sv2 xs2] [_ <-]/=.
+    rewrite (IH _ _ _ _ Fs)//andbT.
+    by apply/check_atom_fresh/Fa.
+  Qed.
+
+  Lemma check_atoms_fresh sP sv bo sv' bo':
+    check_atoms sP bo ->
+      fresh_atoms sv bo = (sv', bo') ->
+      check_atoms sP bo'.
+  Proof.
+    elim: bo bo' sv sv' => //=.
+      move=> > _ [_ <-]//.
+    move=> //= x xs IH bo' sv sv'.
+    case Fs: fresh_atoms => [b' xs'].
+    case Fa: fresh_atom => [b2 a2] + [_ <-]/=.
+    destruct x; move: Fa => /=.
+      move=> [_<-].
+      move=> /orP[] H; apply/orP.
+        by rewrite (all_check_atom_fresh H Fs); left.
+      by right; apply/IH/Fs.
+    case X: fresh_callable => [b3 c'][_<-] /andP[+/IH-/(_ _ _ _ Fs)->].
+    rewrite andbT.
+    by move=> /orP[/tm_is_det_fresh -/(_ _ _ _ X)|/fresh_has_cut-/(_ _ _ _ Fs)]->//; rewrite orbT.
+  Qed.
+
+  Fixpoint mut_excl sig rules :=
+    match rules with
+    | [::] => true
+    | x :: xs => mut_excl_head sig x.(head) rules && mut_excl sig xs
+    end.
+
+End mut_excl.
+
+
+Definition check_program_aux u sig pr := 
+   mut_excl u sig pr && check_rules sig pr.
+
+Definition check_program u pr := 
+   check_program_aux u pr.(sig) pr.(rules).
 
 Section check.
+  Variable u : Unif.
+  (* Variable p : program. *)
+
 
   Fixpoint has_cut A :=
     match A with
@@ -137,9 +300,9 @@ Section check.
     has_cut (big_and l) = has_cut_seq l.
   Proof. by elim: l => //[[|c]] xs IH//=; rewrite IH Bool.andb_diag. Qed.
 
-  Lemma cut_followed_by_det_has_cut {sP l}:
+  (* Lemma cut_followed_by_det_has_cut {sP l}:
       check_atoms sP l -> has_cut_seq l.
-  Proof. rewrite/check_atoms. elim: l => //= -[|c] l _ //=. Qed.
+  Proof. rewrite/check_atoms. elim: l => //= -[|c] l _ //=. Qed. *)
 
   Lemma det_tree_big_and sP L:
     det_tree sP (big_and L) = det_tree_seq sP L.
@@ -157,7 +320,7 @@ Section check.
     move=> [|t] /= l IH.
       move=> /orP [|//].
       by elim: l {IH} => //= x xs IH /andP[->]/IH->.
-    by move=> /[dup] /cut_followed_by_det_has_cut -> /IH-> /[!orbT].
+    by move=> /andP[->]/=.
   Qed.
 
   Lemma no_alt_cutl A: success A -> no_alt (cutl A).
@@ -172,40 +335,6 @@ Section check.
     by rewrite sA HA// HB//no_alt_cutl//.
   Qed.
 
-  Variable u : Unif.
-  Variable p : program.
-
-  Lemma tiki_taka {sP s s3 modes t q pn hd1}:
-    let t' := tm2RC (deref s (Callable2Tm t)) in
-    t' = Some (q, pn) ->
-    tm_is_det sP t ->
-      H u modes q hd1 s = Some s3 ->
-        callable_is_det sP hd1.
-  Proof.
-    move=>/=.
-    elim: modes q pn hd1 t s s3 => //=.
-      move=> []//=k kp hd1 t s1 s2.
-      case: hd1 => //={}k0.
-      case: eqP => //=?; subst k0.
-      move=> ++ [?]; subst.
-      destruct t => //=; last by case: tm2RC => //=[[]].
-      by move=> [->->]/=; rewrite/tm_is_det/=; case: fndP.
-    move=> m //ml IH q pn hd t s1 s2 H1 H2 H3.
-    have {H3}: exists f1 a1 f2 a2,
-      q = Callable_App f1 a1 /\
-      hd = Callable_App f2 a2 /\
-      (obind (matching u a1 a2) (H u ml f1 f2 s1) = Some s2 \/
-      obind (unify u a1 a2) (H u ml f1 f2 s1) = Some s2).
-    by move: H3; destruct m, q, hd => //; repeat eexists; auto.
-    move=> [f1 [a1 [f2 [a2 [?[?]]]]]]; subst.
-    case e: H => //=[s3|]; last by case.
-    move: H2; rewrite/tm_is_det/=.
-    case: t H1 => //= c t.
-    case H : tm2RC => //=[[h1' hp]] [??]?; subst => /=.
-    case X: getS_Callable => //[S] H1/= H2.
-    by apply: IH H _ e; rewrite/tm_is_det X//.
-  Qed.
-
   Lemma check_rules_cons sP x xs : check_rules sP (x :: xs) = check_rule sP (head x) (premises x) && check_rules sP xs.
   by []. Qed.
 
@@ -213,69 +342,6 @@ Section check.
     ((fresh_rule (fresh_rules fv rs).1 r).1, (fresh_rule (fresh_rules fv rs).1 r).2 :: (fresh_rules fv rs).2).
   by simpl; rewrite !push.
 Qed.
-
-  Lemma head_fresh_rule fv r:
-    head (fresh_rule fv r).2 = (fresh_callable fv r.(head)).2.
-  Proof.
-    destruct r; rewrite/fresh_rule/= 1!push.
-    case bc: fresh_atoms => [fv' A']//=.
-  Qed.
-
-  Lemma head_fresh_premises fv r:
-    premises (fresh_rule fv r).2 = (fresh_atoms (fresh_callable fv r.(head)).1 r.(premises)).2.
-  Proof.
-    destruct r; rewrite/fresh_rule/= 1!push.
-    generalize (fresh_callable fv head) => -[{}fv/=b].
-    case FA: fresh_atoms => [b1 a']//=.
-  Qed.
-
-  Lemma callable_is_det_fresh sP fv hd:
-    callable_is_det sP (fresh_callable fv hd).2 =
-      callable_is_det sP hd.
-  Proof.
-    elim: hd fv => //= a Ha t fv.
-    case F: fresh_callable => [fv' a']/=.
-    case F': rename => [fv'' a'']/=.
-    by rewrite -(Ha fv) F.
-  Qed.
-
-  Lemma tm_is_det_comb sP f a:
-    tm_is_det sP (Callable_App f a) = tm_is_det sP f.
-  Proof. by rewrite/tm_is_det/=. Qed.
-  
-  Lemma tm_is_det_fresh sP c c' sv sv':
-    tm_is_det sP c ->
-    fresh_callable sv c = (sv', c') ->
-    tm_is_det sP c'.
-  Proof.
-    elim: c c' sv sv' => //=.
-      by move=> k c' sv sv' + [_ <-]//.
-    move=> f Hf a c' sv sv'.
-    case X: fresh_callable => [sv2 f'].
-    case Y: rename => [sv3 a'] + [_ <-].
-    rewrite !tm_is_det_comb => H.
-    by apply/Hf/X.
-  Qed.
-
-  Lemma fresh_has_cut sv xs sv' xs':
-    has_cut_seq xs -> fresh_atoms sv xs = (sv', xs') -> has_cut_seq xs'.
-  Proof.
-    elim: xs sv xs' sv' => //= x xs IH sv xs' sv'.
-    case Fs: fresh_atoms => [b' a'].
-    case Fa: fresh_atom => [b2 a2]/=+[_<-]/=.
-    move=> /orP [/eqP?|]; subst; first by move: Fa => /=[_<-].
-    by move=> H; rewrite (IH _ _ _ H Fs) orbT.
-  Qed.
-
-  Lemma check_atom_fresh sP x x' sv sv':
-    check_atom sP x ->
-    fresh_atom sv x = (sv', x') ->
-    check_atom sP x'.
-  Proof.
-    destruct x => //=; first by move=> _ [_ <-].
-    case X: fresh_callable => [svE c'] H [_ <-]/=.
-    by apply/tm_is_det_fresh/X.
-  Qed.
 
   Lemma det_tree_fresh sP sv bo:
     det_tree_seq sP bo -> det_tree_seq sP (fresh_atoms sv bo).2.
@@ -288,37 +354,6 @@ Qed.
     by rewrite (fresh_has_cut H Fs) orbT.
   Qed.
 
-  Lemma all_check_atom_fresh sP xs xs' sv sv':
-    all (check_atom sP) xs ->
-    fresh_atoms sv xs = (sv', xs') ->
-    all (check_atom sP) xs'.
-  Proof.
-    elim: xs xs' sv sv' => //=; first by move=> > _ [_ <-].
-    move=> x xs IH xsE sv svE /andP[H1 H2].
-    case Fs: fresh_atoms => [sv' xs'].
-    case Fa: fresh_atom => [sv2 xs2] [_ <-]/=.
-    rewrite (IH _ _ _ _ Fs)//andbT.
-    by apply/check_atom_fresh/Fa.
-  Qed.
-
-  Lemma check_atoms_fresh sP sv bo sv' bo':
-    check_atoms sP bo ->
-      fresh_atoms sv bo = (sv', bo') ->
-      check_atoms sP bo'.
-  Proof.
-    elim: bo bo' sv sv' => //= x xs IH bo' sv sv'.
-    case Fs: fresh_atoms => [b' a'].
-    case Fa: fresh_atom => [b2 a2] + [_ <-]/=.
-    destruct x; move: Fa => /=.
-      move=> [_<-].
-      move=> /orP[] H; apply/orP.
-        by rewrite (all_check_atom_fresh H Fs); left.
-      by right; apply/IH/Fs.
-    case X: fresh_callable => [b3 c'][_<-] H.
-    by apply/IH/Fs.
-  Qed.
-
-
   Lemma select_same2 vx vy q m rs s:
     (select u vx q m rs s).2 = (select u vy q m rs s).2.
   Proof.
@@ -326,40 +361,188 @@ Qed.
     case: H => //=?; rewrite !push//=; f_equal; auto.
   Qed.
 
-  Lemma is_det_no_free_alt {sP t s1 fv}:
-    check_rules sP p.(rules) -> tm_is_det sP t -> 
-      det_tree sP (backchain u p fv s1 t).2.
+  Lemma tm_is_det_tm2RC s s1 c :
+    tm_is_det s c ->
+    exists q qp (kP: qp \in domf s), 
+      tm2RC (deref s1 (Callable2Tm c)) = Some (q, qp) /\ is_det_sig s.[kP].
   Proof.
-    rewrite /backchain/bc.
-    case X: tm2RC => //=[[q qp]].
-    case: p => rules sig1 /=.
+    rewrite/tm_is_det.
+    case CS: getS_Callable => //=[S].
+    elim: c s1 S CS => //= [p|f IH a] s1 S.
+      by case: fndP => //= kP [<-] dS; repeat eexists; eassumption.
+    move=> H DS.
+    have [q[qp [kP [H1 H2]]]] := IH s1 _ H DS.
+    by rewrite H1; repeat eexists; apply: H2.
+  Qed.
+
+  (* Lemma mut_exclP *)
+
+  Lemma check_rulesP s rs c fv s1:
+    check_rules s rs ->
+    tm_is_det s c ->
+    all (fun x => check_atoms s x.2.(premises)) (bc u {| rules := rs; sig := s |} fv c s1).2.
+  Proof.
+    rewrite/bc.
+    case DR: tm2RC => //=[[q p]].
+    case: fndP => //= pP.
+    rewrite push/=.
+    case X: fresh_rules => [fv1 rs']/=.
+    generalize (get_modes_rev q s.[pP]) => md.
+    generalize fv1 => fv2.
+    elim: rs fv2 md rs' s c s1 fv q p {pP} fv1 DR X => //=[|[hd bo] rs IH] fv2 md rs' s c s1 fv q p fv1 DR ++ TD.
+      move=> [_ <-]//.
+    case FS: fresh_rules => [fv3 rs3].
+    case FR: fresh_rule => [fv4 r'][??]/=/andP[H1 H2]; subst.
+    move=> /=.
+    have {}IH := IH _ _ _ _ _ _ _ _ _ _ DR FS H2 TD.
+    case H: H => //=; last by apply: IH.
+    rewrite !push/=.
+    have TD' := tiki_taka DR TD H.
+    move: FR.
+    rewrite/fresh_rule !push/=.
+    case X: fresh_atoms => [fs2 f']/= => -[??]; subst => /=.
+    rewrite /= callable_is_det_fresh in TD'.
+    move: H1; rewrite/check_rule TD'/= => ?.
+    rewrite (check_atoms_fresh _ X)//=.
+    apply: IH.
+  Qed.
+
+  Lemma deref_empty t:
+    deref empty t = t.
+  Proof. by elim: t => //= [v|f -> a ->//]; case: fndP => //=. Qed.
+
+  (* sufficient modes length for callable t *)
+  Fixpoint suff_mode (t:Callable) (m:seq mode) :=
+    match m, t with
+    | [::], Callable_P _ => true
+    | [:: _ & xs], Callable_App x _ => suff_mode x xs
+    | _, _ => false
+    end.
+
+  Lemma HH q' hd qp m s :
+    suff_mode hd m -> tm2RC (Callable2Tm hd) = Some (q', qp) ->
+    H_head u s m q' hd.
+  Proof.
+    elim: hd m s qp q' => //=[p [|_ _]|f Hf a [|m0 ms]]//= s qp q' sm.
+      by move=> [<-]; rewrite //= eqxx.
+    case X: tm2RC => [[q2 qp2]|]//=[??]; subst.
+    have:= Hf _ s _ _ sm X.
+    case: m0 => //=; case: H_head => //= Y _.
+    apply: unif_refl.
+  Qed.
+
+  Lemma tm2RC_rigid_deref c1 d1 h1 d2 h2 s1 s2 fv m c:
+    tm2RC (Callable2Tm c1) = Some (d1, h1) ->
+    H u m d2 (fresh_callable fv c1).2 s1 = Some s2 ->
+    tm2RC c = Some (d2, h2) -> h1 = h2.
+  Proof.
+    elim: c1 d1 h1 d2 h2 s1 s2 fv m c => //=[p|f Hf r] d1 h1 d2 h2 s1 s2 fv m c.
+      move=> [??]; subst.
+      case: m => /=[|[] _]; case: d2 => //p; case: eqP => //=-> _.
+      elim: c h1 h2 => //=[>[<-<-]|]//f Hf a Ha h1 h2.
+      by case X: tm2RC => //[[c1 p1]][//].
+    case H: tm2RC => [[C P]|]//=[??]; subst.
+    rewrite !push/=.
+    have {H}Hf := Hf _ _ _ _ _ _ _ _ _ H.
+    case m => [|[]]//=; case: d2 => //= c1 t1 l1;
+    case H: H => //=[s3]; have {}Hf := Hf _ _ _ _ _ _ _ H;
+    case: c => //= f' a'; case tm: tm2RC => //=[[c' p']]/= + [???]; subst;
+    have:= Hf _ _ tm => //.
+  Qed.
+
+  Lemma tm2RC_get_modes c1 d1 h1 d2 h2 s1 s2 fv m c l:
+    tm2RC (Callable2Tm c1) = Some (d1, h1) ->
+    H u m d2 (fresh_callable fv c1).2 s1 = Some s2 ->
+    tm2RC c = Some (d2, h2) -> 
+      get_modes_rev d1 l = get_modes_rev d2 l.
+  Proof.
+    elim: c1 d1 h1 d2 h2 s1 s2 fv m c l => //=[p|f Hf r] d1 h1 d2 h2 s1 s2 fv m c l.
+      by move=> [??]; subst; case: m => /=[|[] _]; case: d2 => //.
+    case H: tm2RC => [[C P]|]//=[??]; subst.
+    rewrite !push/=.
+    have {H}Hf := Hf _ _ _ _ _ _ _ _ _ _ H.
+    case m => [|[]]//=; case: d2 => //= c1 t1 l1;
+    case H: H => //=[s3]; have {}Hf := Hf _ _ _ _ _ _ _ _ H;
+    case: c => //= f' a'; case tm: tm2RC => //=[[c' p']]/= + [???]; subst;
+    have:= Hf _ _ _ tm => //; case: l => //=;
+    rewrite/get_modes_rev/=/sigtm_rev/sigtm/=!add0n => m1 ml mr IH _;
+    by rewrite !rev_cons/=!map_rcons/= IH.
+  Qed.
+
+  Lemma mut_exclP s rs fv c s1:
+    mut_excl u s rs -> 
+      tm_is_det s c ->
+        all (fun x => has_cut_seq x.2.(premises)) (bc u {|sig:=s; rules := rs|} fv c s1).2.
+  Proof.
+    rewrite/bc.
+    case DR: tm2RC => //=[[q p]].
+    case: fndP => //= pP.
+    rewrite push/=.
+    case X: fresh_rules => [fv1 rs']/=.
+    generalize fv1 => fv2.
+    elim: rs fv2 rs' s c s1 fv q p pP fv1 DR X => //=[|[hd bo] rs IH] fv2 rs' s c s1 fv q p pP fv1 DR ++ TD.
+      move=> [_ <-]//.
+    case FS: fresh_rules => [fv3 rs3].
+    case FR: fresh_rule => [fv4 r'][??]/=/andP[H1 H2]; subst.
+    move=> /=.
+    have {}IH := IH _ _ _ _ _ _ _ _ _ _ DR FS H2 TD.
+    case H: H => //=[s2|]; rewrite !(IH,push)//=IH andbT.
+    have TD' := tiki_taka DR TD H.
+    move: FR.
+    rewrite/fresh_rule !push/=.
+    case X: fresh_atoms => [fs2 f']/= => -[??]; subst => /=.
+    simpl in H.
+    rewrite /= callable_is_det_fresh in TD'.
+    move: H1; rewrite/check_rule/mut_excl_head/=.
+    have [q'[qp[qP[H3 H4]]]] := tm_is_det_tm2RC empty TD'.
+    rewrite deref_empty in H3.
+    rewrite H3 in_fnd H4 {IH FS rs3 fv2}.
+    case: ifP => /=.
+      move=> _ /andP[H5].
+      by have:= fresh_has_cut H5 X.
+    move=> H1.
+    exfalso.
+    apply: Bool.eq_true_false_abs H1.
+    apply: HH (H3).
+    have ?:= tm2RC_rigid_deref H3 H DR; subst.
+    rewrite (bool_irrelevance qP pP).
+    rewrite (tm2RC_get_modes _ H3 H DR).
+    move: H.
+    generalize (get_modes_rev q s.[pP]); clear => l.
+    elim: l hd q s1 s2 fv3 => //=.
+      move=> hd []//= p s1 s2 fv; case fc: fresh_callable => [fv' [p'|]]/=//.
+      case: eqP => //? [?]; subst.
+      by case: hd fc => //= c t; rewrite !push.
+    move=> m l IH hd q s1 s2 fv.
+    case: m; case: q => //= c t; case fc: fresh_callable => [fv' [|f a]]//=;
+    case H: H => [s3|]//=; move: fc; case: hd => //=[f' a']; rewrite !push;
+    move=> [???]; subst => H1; apply: IH H.
+  Qed.
+
+
+  Lemma is_det_no_free_alt pr c sv s1:
+    check_program u pr -> tm_is_det (sig pr) c -> 
+    det_tree (sig pr) (backchain u pr sv s1 c).2.
+  Proof.
+    rewrite /backchain/bc/check_program/check_program_aux.
+    case: pr => rs s/= => /andP[].
+    case X: tm2RC => //=[[q qp]]; rewrite !push/=.
     case: fndP => //= kP.
-    generalize (get_modes_rev q sig1.[kP]).
-    clear kP sig1 p => l.
-    rewrite !push/=.
-    generalize (fresh_rules fv rules).1.
-    elim: rules s1 t q qp X fv l => //.
-    move=> [] hd bo rules IH s t q qp X fv l/=f /andP[ck1 ck2] dett.
-    have {}IH := IH _ _ _ _ X _ _ _ ck2 dett.
-    rewrite !push/=.
-    case H: H => /= [s2|]; last first.
-      by rewrite (select_same2 _ ((fresh_rules fv rules).1)).
-    have Hx := tiki_taka X dett H.
-    rewrite head_fresh_rule/=callable_is_det_fresh in Hx.
-    move/orP: ck1 => []; first by rewrite Hx.
-    rewrite !push/=.
-    have {IH}:= IH fv l f.
-    rewrite head_fresh_premises/=.
-    case S: select => [fv' [|[r0 s0] rs]]/=; rewrite det_tree_big_and.
-      move => _ /cut_followed_by_det_nfa_and.
-      by move=> /det_tree_fresh->.
-    move=> Ha Hb.
-    have ? : check_atoms sP (fresh_atoms (fresh_callable (fresh_rules fv rules).1 hd).1 bo).2.
-      case W: fresh_atoms.
-      by apply/check_atoms_fresh/W.
-    rewrite cut_followed_by_det_nfa_and//.
-    rewrite has_cut_seq_has_cut_big_and//.
-    rewrite (@cut_followed_by_det_has_cut sP)//=.
+    move=> ++ H.
+    have [q'[qp' [H1 [H2 H3]]]] := tm_is_det_tm2RC s1 H.
+    (* case FR: fresh_rules => [fv2 rs']. *)
+    (* case SL: select => [fv3 [|[s0 [hd pm]] rs2]]//=. *)
+    move=> ME CR.
+    have := mut_exclP sv s1 ME H.
+    have := check_rulesP sv s1 CR H.
+    rewrite/bc X/= in_fnd.
+    case: fresh_rules => [a rs'].
+    case: select => /= _.
+    move=> [|[_ + {ME CR}rs]]//=; clear.
+    elim: rs => //=[|[s0 r0] rs IH] [h b]/=/andP[CH CB] /andP[CuH CuB];
+    rewrite det_tree_big_and cut_followed_by_det_nfa_and//=.
+    rewrite has_cut_seq_has_cut_big_and CuH.
+    by apply: IH.
   Qed.
 
   Lemma has_cut_success {A}:
@@ -376,14 +559,11 @@ Qed.
     success A -> has_cut A = false.
   Proof. by apply/contraTF => /has_cut_success->. Qed.
 
-  Lemma step_has_cut_help sv A s: 
+  Lemma step_has_cut_help p sv A s: 
     has_cut A -> has_cut (step u p sv s A).2 \/ is_cb (step u p sv s A).1.2.
   Proof.
     elim: A s sv; try by move=> /=; auto.
     - by move=> []//=; auto.
-    (* - move=> A HA s1 B HB s sv /=/andP[kA kB].
-      by rewrite !push is_ko_step //=kA; left.
-    - by move=> s1 B HB s sv /= kB; rewrite !push is_ko_step//=; auto. *)
     - move=> A HA B0 B HB s sv /=.
       rewrite !push/= => /orP[].
         move=> cA; rewrite has_cut_success//=.
@@ -395,15 +575,15 @@ Qed.
       by rewrite cB; rewrite orbT; auto.
   Qed.
 
-  Lemma step_keep_cut A s sv: 
+  Lemma step_keep_cut p A s sv: 
     has_cut A -> is_cb (step u p sv s A).1.2 = false -> 
       has_cut (step u p sv s A).2.
-  Proof. move/step_has_cut_help => /(_ sv s)[]//->//. Qed.
+  Proof. move/step_has_cut_help => /(_ p sv s)[]//->//. Qed.
 
   Lemma succ_failF_no_alt A: success A = false -> failed A = false -> no_alt A = false.
   Proof. by rewrite/no_alt => -> /failedF_next_alt ->//. Qed.
 
-  Lemma no_alt_det_tree sP fv c s:
+  Lemma no_alt_det_tree p sP fv c s:
     no_alt (backchain u p fv s c).2 -> det_tree sP (backchain u p fv s c).2.
   Proof.
     rewrite/backchain !push/=.
@@ -411,24 +591,25 @@ Qed.
     rewrite/no_alt/=.
     rewrite next_alt_big_or//.
   Qed.
-  Lemma step_no_free_alt {sP sv s1 A r} : 
-    check_program sP p -> det_tree sP A -> 
-      step u p sv s1 A = r ->
-        det_tree sP r.2.
+
+  Lemma step_no_free_alt pr sv s1 A r: 
+    check_program u pr -> det_tree pr.(sig) A -> 
+      step u pr sv s1 A = r ->
+        det_tree pr.(sig) r.2.
   Proof.
     move=> H + <-; clear r.
     elim_tree A s1.
-    - by case: t => [|c]//=; rewrite push => /is_det_no_free_alt->//.
+    - case: t => [|c]//=; rewrite !push/=.
+      by apply: is_det_no_free_alt.
     - move=>/= /andP[fA]; rewrite !push/= HA//=.
       case: ifP => //= cA; last by move=> /eqP->; rewrite !if_same.
       rewrite !fun_if => /[dup] Hx ->; do 2 case: ifP => //=.
-      by move=> Hy Hz; rewrite step_keep_cut in Hz.
+      by move=> H1; rewrite (step_keep_cut _ H1).
     - by rewrite /=!push; move=> /HB/=->.
     - rewrite step_and/= => /andP[dB].
-      (* rewrite/no_alt. *)
       set sB:= step _ _ _ _ B.
       set sA:= step _ _ _ _ A.
-        rewrite (fun_if (det_tree sP)).
+      rewrite (fun_if (det_tree (sig pr))).
       case SA: success.
         case : (ifP (is_cb _)) => /=; rewrite {}HB//=.
           by rewrite det_tree_cutl//no_alt_cutl//= andbT.
@@ -531,22 +712,22 @@ Qed.
       by case/orP=> [/HA/(_ nA)->//|/andP[? ->]]; rewrite orbT.
   Qed.
 
-  Lemma step_next_alt_failedF {sP sv sv' A B C s b}:
-    check_program sP p ->
-      det_tree sP A -> step u p sv s A = (sv', Failed, B) ->
-        next_alt b B = Some (C) -> det_tree sP C.
+  Lemma step_next_alt_failedF p sv sv' A B C s b:
+    check_program u p ->
+      det_tree p.(sig) A -> step u p sv s A = (sv', Failed, B) ->
+        next_alt b B = Some (C) -> det_tree p.(sig) C.
   Proof.
     move=> H1 H2 H3 H4.
     have /= H5 := step_no_free_alt H1 H2 H3.
     by have:= no_free_alt_next_alt H5 H4.
   Qed.
 
-  Definition is_det A := forall b s sv s' B fv',
+  Definition is_det u p A := forall b s sv s' B fv',
     run u p sv s A s' B b fv' -> B = None.
 
-  Lemma run_next_alt {sP A}: 
-    check_program sP p -> 
-      det_tree sP A -> is_det A.
+  Lemma run_next_alt p A: 
+    check_program u p -> 
+      det_tree p.(sig) A -> is_det u p A.
   Proof.
     rewrite/is_det.
     move=> H1 H2 b s sv s' B ? H3.
@@ -556,9 +737,9 @@ Qed.
     - by apply/IH/no_free_alt_next_alt/nA.
   Qed.
 
-  Lemma main {sP t}:
-    check_program sP p -> tm_is_det sP t -> 
-      is_det (TA (call t)).
+  Lemma main p t:
+    check_program u p -> tm_is_det p.(sig)  t -> 
+      is_det u p (TA (call t)).
   Proof.
     move=> H1 fA HA.
     apply: run_next_alt H1 _ HA.
@@ -567,18 +748,32 @@ Qed.
 
   Print Assumptions  main.
   
-  Section tail_cut.
+  (* Section tail_cut.
 
     Definition tail_cut (r : R) :=
     match r.(premises) with [::] => false | x :: xs => last x xs == cut end.
     
     Definition AllTailCut p := (all tail_cut (rules p)).
 
-    Lemma cut_in_prem_tail_cut sP: AllTailCut p -> check_program sP p.
+    Lemma cut_in_prem_tail_cut : AllTailCut p -> check_program u p.
     Proof.
+      case: p; rewrite/AllTailCut/check_program/=.
+      move=> rules sig H; apply/andP; split.
+        elim: rules sig H => //= x xs IH sig /andP[H1 H2].
+        rewrite IH//andbT.
+        rewrite/mut_excl_head/=.
+        case: tm2RC => [[c p']|]//; case: fndP => //= kP.
+        case: ifP => //= HD.
+        case: x H1 => /= hd pm; clear -H2.
+        rewrite/tail_cut/=.
+        elim: pm hd xs H2 => //= x xs IH.
+        generalize sig.[kP].
+        move : (sig.[kP]) => /=.
+      move=> H; apply/andP; split. move: H; case: p.
       rewrite /AllTailCut /check_program.
       rewrite /tail_cut /check_rules.
       remember (rules p) as RS.
+
       apply: sub_all => r; clear.
       rewrite /check_rule.
       case X: callable_is_det => //=.
@@ -595,8 +790,8 @@ Qed.
       move=> /(cut_in_prem_tail_cut sP).
       apply main.
     Qed.
-  End tail_cut.
+  End tail_cut. *)
 
-  Print Assumptions tail_cut_is_det.
+  (* Print Assumptions tail_cut_is_det. *)
 
 End check.
